rocq-brick-libstdcpp/test/optional/check_named_lvalue_roundtrip.v
@@ -32,22 +32,35 @@ Section with_cpp.
       \post emp
     ).
   
-  Lemma check_named_lvalue_roundtrip_proof :
-    verify[clients_cpp.module] "check_named_lvalue_roundtrip(unsigned char)".
+  
+#[program] Definition optional_uint8_R_engaged_byte_C
+    (o p : ptr) (q : cQp.t) (b : Z) :=
+  \cancelx
+  \consuming o |-> optional_uint8.R q (Some b) (Some p)
+  \proving p |-> ucharR q b
+  \end.
+Next Obligation.
+  intros.
+  rewrite optional_uint8.R.unlock.
+  rewrite _at_sep _at_pureR.
+  go.
+Qed.
+#[local] Hint Resolve optional_uint8_R_engaged_byte_C : br_hints.
+#[local] Hint Resolve fractional.UNSAFE_read_prim_learn : sl_opacity.
+#[local] Instance optional_uint8_R_read_learn :
+  AtLearnEq3 optional_uint8.R := ltac:(solve_learnable).
 
-    try rewrite /optional_uint8_value_lvalue_ctor_spec.
-    try rewrite /optional_uint8_has_value_template_spec.
-    try rewrite /optional_uint8_deref_const_lvalue_template_spec.
-    try rewrite /optional_uint8_destructor_template_spec.
-    try rewrite /assert_fail_unreachable_spec.
+Lemma check_named_lvalue_roundtrip_proof :
+  verify[clients_cpp.module] "check_named_lvalue_roundtrip(unsigned char)".
 Proof using MOD.
-    rewrite /optional_uint8_value_lvalue_ctor_spec
-      /optional_uint8_has_value_spec
-      /optional_uint8_deref_const_lvalue_spec
-      /optional_uint8_destructor_spec.
-    verify_spec.
-    
-repeat first [ progress (go) | iExists _; iFrame | rewrite (AutoUnlocking.unfold_eq (Unfoldable := optional_uint8.R_unfoldable _ _ _ _ _ _ _)) ].
+  rewrite /optional_uint8_value_lvalue_ctor_spec
+    /optional_uint8_has_value_spec
+    /optional_uint8_deref_const_lvalue_spec
+    /optional_uint8_destructor_spec
+    /assert_fail_unreachable_spec.
+  verify_spec; go.
+  Unshelve.
+  all: ego; go.
+Qed.
 
-  Qed.
 End with_cpp.
