rocq-brick-libstdcpp/test/optional/empty_deref_zero_rejected.v
@@ -36,41 +36,60 @@ Section with_cpp.
   cpp.spec "empty_deref_zero_rejected()"
     from empty_deref_zero_rejected_cpp.source
     as empty_deref_zero_rejected_spec with (\post emp).
-  Lemma empty_deref_zero_rejected_proof :
-    denoteModule empty_deref_zero_rejected_cpp.source |--
-      (▷ optional_uint8_nullopt_ctor_spec **
-       ▷ optional_uint8_deref_const_lvalue_spec **
-       ▷ optional_uint8_destructor_spec -*
-       empty_deref_zero_rejected_spec).
-  Proof using MOD.
-    rewrite /optional_uint8_nullopt_ctor_spec
-      /optional_uint8_deref_const_lvalue_spec
-      /optional_uint8_destructor_spec.
-    verify_spec.
-    
+#[local] Hint Resolve fractional.UNSAFE_read_prim_learn : sl_opacity.
+#[local] Instance optional_uint8_R_read_learn :
+  AtLearnEq3 optional_uint8.R := ltac:(solve_learnable).
 
 
-repeat first
-      [ progress (go)
-      | iExists _; iFrame
-      | rewrite (AutoUnlocking.unfold_eq (Unfoldable := optional_uint8.R_unfoldable _ _ _ _ _ _ _))
-      | (iApply wp_init_constructor_inline;
-          [exact (InlineMe _) | go |])
-      | (iApply destroy_val_named_inline;
-          [exact (InlineMe _) | go |])
-      ].
+Lemma empty_deref_zero_rejected_proof :
+  denoteModule empty_deref_zero_rejected_cpp.source |--
+    (▷ optional_uint8_nullopt_ctor_spec **
+     ▷ optional_uint8_deref_const_lvalue_spec **
+     ▷ optional_uint8_destructor_spec -*
+     empty_deref_zero_rejected_spec).
+Proof using MOD.
+  rewrite /optional_uint8_nullopt_ctor_spec
+    /optional_uint8_deref_const_lvalue_spec
+    /optional_uint8_destructor_spec
+    /assert_fail_unreachable_spec
+    /nullopt_copy_ctor_spec
+    /nullopt_destructor_spec.
+  verify_spec; go.
+  Unshelve.
+  all: try exact None.
+  all: ego; go.
+  all: try (
+    iApply wp_init_constructor_inline;
+      [exact (InlineMe _) | go |]
+  ).
+  all: go.
+  all: try (
+    iApply destroy_val_named_inline;
+      [exact (InlineMe _) | go |]
+  ).
+  all: go.
+  Unshelve.
+  all: try exact (Vint 0).
+  all: try exact (1$c)%cQp.
+  all: ego; go.
+  all: try (
+    rewrite !optional_uint8.R.unlock !_at_sep !_at_pureR;
+    wname [ (o_addr |-> optional_uint8.spineR _ None) ] "Hempty";
+    wname [ (o_addr |-> optional_uint8.spineR _ (Some _)) ] "Hengaged";
+    iDestruct (observe_2 [| (None : option ptr) = Some _ |]
+      with "Hempty Hengaged") as %Hbad;
+    discriminate Hbad
+  ).
 
-Unshelve. all: try exact None.
-repeat first
-      [ progress (go)
-      | iExists _; iFrame
-      | rewrite (AutoUnlocking.unfold_eq (Unfoldable := optional_uint8.R_unfoldable _ _ _ _ _ _ _))
-      | (iApply wp_init_constructor_inline;
-          [exact (InlineMe _) | go |])
-      | (iApply destroy_val_named_inline;
-          [exact (InlineMe _) | go |])
-      ].
+  Unshelve.
+  all: try exact (Vint 0).
+  all: try exact (1$c)%cQp.
+  all: try (ego; go).
 Fail Qed.
 Abort.
+
+
+
+  
 
 End with_cpp.
